### Additivity

Consider any $\mathcal{A}, \mathcal{B} \subseteq \mathcal{X}$ s.t. 
$\mathcal{A} \cap \mathcal{B} = \emptyset$.

Note that $\mathcal{A} = {a_1, \ldots, a_K}$ and $\mathcal{B} = {b_1, \ldots, b_L}$.

Define $c_1 = a_1, \ldots, c_K = a_K, c_{K+1} = b_1, \ldots, c_{K+L} = b_L$.

---

We first show that $P_X(\mathcal{A}) = \sum_{k=1}^L P_X( a_k )$.
$$
\begin{aligned}
P_X(\mathcal{A}) 
 &= P_X\left( \bigcup_{k=1}^K a_k \right) \\
 &= P\left( \bigcup_{k=1}^K \{ s_k \in \mathcal{S} : X(s_k) == a_k \} \right) 
  \quad (\text{definition of }P_X) \\
 &= \sum_{k=1}^K P\left( \{s_k \in \mathcal{S} : X(s_k) == a_k \} \right)
  \quad (\text{additivity of }P) \\
 &= \sum_{k=1}^K P_X( a_k )
  \quad (\text{definition of }P_X)
\end{aligned}
$$

By the same derivation as above, we can also show $P_X(\mathcal{B}) = \sum_{l=1}^L P_X( b_l )$.

---

$$
\begin{aligned}
P_X \left( \mathcal{A} \cup \mathcal{B} \right)
 &= P_X \left( \left(\bigcup_{k=1}^K a_k\right) \cup \left(\bigcup_{l=1}^L b_k\right) \right)
 &= P\left(
   \bigcup_{k=1}^K \{s_k \in \mathcal{S} : X(s_k) == a_k \} \cup 
   \bigcup_{l=1}^L \{s_k \in \mathcal{S} : X(s_k) == b_l \}
  \right) 
  \quad (\text{definition of }P_X) \\
 &= P\left(
   \bigcup_{k=1}^{K+L} \{s_k \in \mathcal{S} : X(s_k) == c_k \}
  \right)
  \quad (\text{definition of }c_k) \\
 &= \sum_{k=1}^{K+L} P\left( \{s_k \in \mathcal{S} : X(s_k) == c_k \} \right)
  \quad (\text{additivity of }P) \\
 &= \sum_{k=1}^{K+L} P_X( c_k )
  \quad (\text{definition of }P_X) \\
 &= \left( \sum_{k=1}^{K} P_X( c_k ) \right) 
  + \left( \sum_{k=K+1}^{K+L} P_X( c_k ) \right) \\
 &= \left( \sum_{k=1}^{K} P_X( a_k ) \right) 
  + \left( \sum_{l=1}^{L} P_X( b_k ) \right)
  \quad (\text{definition of }c_k) \\
 &= P_X(\mathcal{A}) + P_X(\mathcal{B}) .
\end{aligned}
$$

---

Therefore, for any $\mathcal{A}, \mathcal{B} \subseteq \mathcal{X}$
s.t. $\mathcal{A} \cap \mathcal{B} = \emptyset$,
$$
P_X \left( \mathcal{A} \cup \mathcal{B} \right) = 
 P_X \left(\mathcal{A}\right) + P_X \left(\mathcal{A}\right) .
$$

The same derivation holds for any pair-wise disjoint subsets of $\mathcal{X}$.  $\blacksquare$
